compiler/src/toRocq.ml
@@ -2,150 +2,153 @@ open Utils
 open Prog
 open Wsize
 open Operators
-
 module F = Format
-module SS = Set.Make(String)
+module SS = Set.Make (String)
 
-let sanitize_c c =
-  if (c >= 'a' && c <= 'z') || (c >= 'A' && c <= 'Z') || (c >= '0' && c <= '9') then c else '_'
+(* -------------------------------------------------------------------------- *)
+(* Identifiers *)
 
+(* The lexer only allows these for identifiers, but the compiler may introduce
+   names with other characters (e.g., periods). *)
+let is_ident_c c =
+  (c >= 'a' && c <= 'z')
+  || (c >= 'A' && c <= 'Z')
+  || (c >= '0' && c <= '9')
+  || c = '_'
+
+let sanitize_c c = if is_ident_c c then c else '_'
 let sanitize_s = String.map sanitize_c
-
-let sanitize_v v = sanitize_s (v.v_name ^ string_of_uid v.v_id)
-let sanitize_fn fn = sanitize_s (fn.fn_name ^ string_of_uid fn.fn_id)
-
-(* Name for variables. *)
+let sanitize_v v = sanitize_s (v.v_name ^ "_" ^ string_of_uid v.v_id)
+let sanitize_fn fn = sanitize_s (fn.fn_name ^ "_" ^ string_of_uid fn.fn_id)
 let pp_var fmt v = F.fprintf fmt "%s" (sanitize_v v)
+let pp_var_i fmt v = pp_var fmt (L.unloc v)
+let pp_gvar fmt v = pp_var_i fmt v.gv
 
-(* Name for functions. *)
+(* We define a Rocq [gvar] under the name [pp_var]. To access the [var_i] and
+   [var], we use projections. *)
+let pp_gv_var fmt v = F.fprintf fmt "%a.(gv)" pp_var v
+let pp_gv_var_i fmt v = F.fprintf fmt "%a.(gv)" pp_var_i v
+let pp_v_var_var fmt v = F.fprintf fmt "%a.(gv).(v_var)" pp_var v
 let pp_fn fmt fn = F.fprintf fmt "%s" (sanitize_fn fn)
-
-(* Name for function declarations. *)
 let pp_fd_name fmt fn = F.fprintf fmt "fd_%a" pp_fn fn
 
+(* -------------------------------------------------------------------------- *)
+(* Rocq helpers *)
 
-(* -------------------------------------------------------------------- *)
-(* Helpers *)
+let pp_newline fmt = F.fprintf fmt "@ "
 
-let pp_list pp fmt =
-  let pp_sep fmt () = F.fprintf fmt ";@ " in
-  F.fprintf fmt "[:: @[<hov>%a@] ]" (F.pp_print_list ~pp_sep pp)
+let pp_rocq_seq pp fmt xs =
+  match xs with
+  | [] -> F.fprintf fmt "[::]"
+  | _ ->
+      let pp_sep fmt () =
+        F.pp_print_break fmt 0 2;
+        F.fprintf fmt "; "
+      in
+      F.fprintf fmt "@[<hv>[:: %a ]@]" (F.pp_print_list ~pp_sep pp) xs
 
-let pp_option pp =
+let pp_rocq_option pp =
   let none fmt () = F.fprintf fmt "None" in
   let some fmt a = F.fprintf fmt "(Some %a)" pp a in
   F.pp_print_option ~none some
 
-let pp_string fmt s =
-  F.fprintf fmt "%S" s
-
-let pp_z fmt z =
-  F.fprintf fmt "(%a)%%Z" Z.pp_print z
+let pp_string fmt s = F.fprintf fmt "%S" s
+let pp_z fmt z = F.fprintf fmt "(%a)%%Z" Z.pp_print z
 
 let pp_positive fmt p =
   F.fprintf fmt "%a%%positive" Z.pp_print (Conv.z_of_pos p)
 
-(* -------------------------------------------------------------------- *)
-(* Wsize *)
+let pp_separator fmt pp x =
+  F.fprintf fmt
+    "(* \
+     -------------------------------------------------------------------------- \
+     *)@ ";
+  F.fprintf fmt "(* %a *)@ " pp x;
+  pp_newline fmt
+
+let pp_separator_s fmt s = pp_separator fmt F.pp_print_string s
+let pp_comment fmt s = F.fprintf fmt "(* %s *)@ " s
+
+let pp_rocq_definition_gen fmt pp_lhs lhs pp_type ty pp_rhs rhs =
+  F.fprintf fmt "@[<hv 2>Definition %a : %a :=@ %a@].@ " pp_lhs lhs pp_type ty
+    pp_rhs rhs
+
+let pp_rocq_definition fmt pp_lhs lhs ty pp_rhs rhs =
+  pp_rocq_definition_gen fmt pp_lhs lhs F.pp_print_string ty pp_rhs rhs
+
+let pp_rocq_record pp fmt x = F.fprintf fmt "@[<v 0>{|@[<v 0>@ %a@]@ |}@]" pp x
+
+(* -------------------------------------------------------------------------- *)
+(* Jasmin *)
 
 let pp_wsize fmt = function
-  | U8   -> F.fprintf fmt "U8"
-  | U16  -> F.fprintf fmt "U16"
-  | U32  -> F.fprintf fmt "U32"
-  | U64  -> F.fprintf fmt "U64"
+  | U8 -> F.fprintf fmt "U8"
+  | U16 -> F.fprintf fmt "U16"
+  | U32 -> F.fprintf fmt "U32"
+  | U64 -> F.fprintf fmt "U64"
   | U128 -> F.fprintf fmt "U128"
   | U256 -> F.fprintf fmt "U256"
 
-(* -------------------------------------------------------------------- *)
-(* Signedness *)
-
 let pp_signedness fmt = function
-  | Signed   -> F.fprintf fmt "Signed"
+  | Signed -> F.fprintf fmt "Signed"
   | Unsigned -> F.fprintf fmt "Unsigned"
 
-(* -------------------------------------------------------------------- *)
-(* Types *)
-
 let pp_atype fmt = function
-  | Bty Bool  -> F.fprintf fmt "abool"
-  | Bty Int   -> F.fprintf fmt "aint"
+  | Bty Bool -> F.fprintf fmt "abool"
+  | Bty Int -> F.fprintf fmt "aint"
   | Bty (U ws) -> F.fprintf fmt "(aword %a)" pp_wsize ws
   | Arr (ws, n) -> F.fprintf fmt "(aarr %a %d)" pp_wsize ws n
 
-(* -------------------------------------------------------------------- *)
-(* Aligned *)
-
 let pp_aligned fmt = function
-  | Memory_model.Aligned   -> F.fprintf fmt "Aligned"
+  | Memory_model.Aligned -> F.fprintf fmt "Aligned"
   | Memory_model.Unaligned -> F.fprintf fmt "Unaligned"
 
-(* -------------------------------------------------------------------- *)
-(* Array access *)
-
 let pp_arr_access fmt = function
-  | Warray_.AAscale  -> F.fprintf fmt "AAscale"
+  | Warray_.AAscale -> F.fprintf fmt "AAscale"
   | Warray_.AAdirect -> F.fprintf fmt "AAdirect"
 
-(* -------------------------------------------------------------------- *)
-(* Assgn tag *)
-
 let pp_assgn_tag fmt = function
-  | Expr.AT_none    -> F.fprintf fmt "AT_none"
-  | Expr.AT_keep    -> F.fprintf fmt "AT_keep"
-  | Expr.AT_rename  -> F.fprintf fmt "AT_rename"
-  | Expr.AT_inline  -> F.fprintf fmt "AT_inline"
+  | Expr.AT_none -> F.fprintf fmt "AT_none"
+  | Expr.AT_keep -> F.fprintf fmt "AT_keep"
+  | Expr.AT_rename -> F.fprintf fmt "AT_rename"
+  | Expr.AT_inline -> F.fprintf fmt "AT_inline"
   | Expr.AT_phinode -> F.fprintf fmt "AT_phinode"
 
-(* -------------------------------------------------------------------- *)
-(* Align *)
-
 let pp_align fmt = function
-  | Expr.Align   -> F.fprintf fmt "Align"
+  | Expr.Align -> F.fprintf fmt "Align"
   | Expr.NoAlign -> F.fprintf fmt "NoAlign"
 
-(* -------------------------------------------------------------------- *)
-(* Direction *)
-
 let pp_dir fmt = function
-  | Expr.UpTo   -> F.fprintf fmt "UpTo"
+  | Expr.UpTo -> F.fprintf fmt "UpTo"
   | Expr.DownTo -> F.fprintf fmt "DownTo"
 
-let pp_var_i fmt v = pp_var fmt (L.unloc v)
-
-let pp_gvar fmt v = pp_var_i fmt v.gv
-
-(* -------------------------------------------------------------------- *)
-(* Op_kind *)
-
 let pp_op_kind fmt = function
-  | Op_int  -> F.fprintf fmt "Op_int"
+  | Op_int -> F.fprintf fmt "Op_int"
   | Op_w ws -> F.fprintf fmt "(Op_w %a)" pp_wsize ws
-
-(* -------------------------------------------------------------------- *)
-(* Cmp_kind *)
 
 let pp_cmp_kind fmt = function
   | Cmp_int -> F.fprintf fmt "Cmp_int"
   | Cmp_w (s, ws) -> F.fprintf fmt "(Cmp_w %a %a)" pp_signedness s pp_wsize ws
 
-(* -------------------------------------------------------------------- *)
-(* Velem / pelem *)
-
 let pp_pelem fmt = function
-  | PE1   -> F.fprintf fmt "PE1"
-  | PE2   -> F.fprintf fmt "PE2"
-  | PE4   -> F.fprintf fmt "PE4"
-  | PE8   -> F.fprintf fmt "PE8"
-  | PE16  -> F.fprintf fmt "PE16"
-  | PE32  -> F.fprintf fmt "PE32"
-  | PE64  -> F.fprintf fmt "PE64"
+  | PE1 -> F.fprintf fmt "PE1"
+  | PE2 -> F.fprintf fmt "PE2"
+  | PE4 -> F.fprintf fmt "PE4"
+  | PE8 -> F.fprintf fmt "PE8"
+  | PE16 -> F.fprintf fmt "PE16"
+  | PE32 -> F.fprintf fmt "PE32"
+  | PE64 -> F.fprintf fmt "PE64"
   | PE128 -> F.fprintf fmt "PE128"
 
 let pp_velem fmt = function
-  | VE8  -> F.fprintf fmt "VE8"
+  | VE8 -> F.fprintf fmt "VE8"
   | VE16 -> F.fprintf fmt "VE16"
   | VE32 -> F.fprintf fmt "VE32"
   | VE64 -> F.fprintf fmt "VE64"
+
+let pp_wrepr ws fmt n = F.fprintf fmt "wrepr %a %a" pp_wsize ws pp_z n
+let pp_word_ty fmt ws = F.fprintf fmt "word %a" pp_wsize ws
+let pp_word ws fmt w = F.fprintf fmt "%a" (pp_wrepr ws) (Conv.z_of_word ws w)
 
 (* -------------------------------------------------------------------- *)
 (* Helpers for printing Rocq constructors with their arguments.
@@ -154,15 +157,12 @@ let pp_velem fmt = function
 (* TODO fmt should go as the first argument *)
 
 let pp_bare name fmt = F.fprintf fmt "%s" name
-
-let pp_with_ws name fmt ws =
-  F.fprintf fmt "(%s %a)" name pp_wsize ws
+let pp_with_ws name fmt ws = F.fprintf fmt "(%s %a)" name pp_wsize ws
 
 let pp_with_ws2 name fmt (ws1, ws2) =
   F.fprintf fmt "(%s %a %a)" name pp_wsize ws1 pp_wsize ws2
 
-let pp_ve name fmt ve =
-  F.fprintf fmt "(%s %a)" name pp_velem ve
+let pp_ve name fmt ve = F.fprintf fmt "(%s %a)" name pp_velem ve
 
 let pp_ve_ws name fmt (ve, ws) =
   F.fprintf fmt "(%s %a %a)" name pp_velem ve pp_wsize ws
@@ -172,38 +172,39 @@ let pp_s_ws name fmt (s, ws) =
 
 let pp_reg_kind fmt = function
   | Wsize.Normal -> F.fprintf fmt "Normal"
-  | Wsize.Extra  -> F.fprintf fmt "Extra"
+  | Wsize.Extra -> F.fprintf fmt "Extra"
 
 let pp_rk_ws name fmt (rk, ws) =
   F.fprintf fmt "(%s %a %a)" name pp_reg_kind rk pp_wsize ws
 
 let pp_ve_ws_ve_ws name fmt (ve1, ws1, ve2, ws2) =
-  F.fprintf fmt "(%s %a %a %a %a)" name
-    pp_velem ve1 pp_wsize ws1 pp_velem ve2 pp_wsize ws2
+  F.fprintf fmt "(%s %a %a %a %a)" name pp_velem ve1 pp_wsize ws1 pp_velem ve2
+    pp_wsize ws2
 
 (* -------------------------------------------------------------------- *)
-(* Unary operators *)
+(* Operators *)
 
 let pp_wiop1 fmt = function
-  | WIwint_of_int ws  -> F.fprintf fmt "(WIwint_of_int %a)" pp_wsize ws
-  | WIint_of_wint ws  -> F.fprintf fmt "(WIint_of_wint %a)" pp_wsize ws
+  | WIwint_of_int ws -> F.fprintf fmt "(WIwint_of_int %a)" pp_wsize ws
+  | WIint_of_wint ws -> F.fprintf fmt "(WIint_of_wint %a)" pp_wsize ws
   | WIword_of_wint ws -> F.fprintf fmt "(WIword_of_wint %a)" pp_wsize ws
   | WIwint_of_word ws -> F.fprintf fmt "(WIwint_of_word %a)" pp_wsize ws
-  | WIwint_ext (szo, szi) -> F.fprintf fmt "(WIwint_ext %a %a)" pp_wsize szo pp_wsize szi
-  | WIneg ws          -> F.fprintf fmt "(WIneg %a)" pp_wsize ws
+  | WIwint_ext (szo, szi) ->
+      F.fprintf fmt "(WIwint_ext %a %a)" pp_wsize szo pp_wsize szi
+  | WIneg ws -> F.fprintf fmt "(WIneg %a)" pp_wsize ws
 
 let pp_sop1 fmt = function
-  | Oword_of_int ws    -> F.fprintf fmt "(Oword_of_int %a)" pp_wsize ws
-  | Oint_of_word (s,ws) -> F.fprintf fmt "(Oint_of_word %a %a)" pp_signedness s pp_wsize ws
-  | Osignext (szo, szi) -> F.fprintf fmt "(Osignext %a %a)" pp_wsize szo pp_wsize szi
-  | Ozeroext (szo, szi) -> F.fprintf fmt "(Ozeroext %a %a)" pp_wsize szo pp_wsize szi
-  | Onot                -> F.fprintf fmt "Onot"
-  | Olnot ws           -> F.fprintf fmt "(Olnot %a)" pp_wsize ws
-  | Oneg k             -> F.fprintf fmt "(Oneg %a)" pp_op_kind k
-  | Owi1 (sg, o)       -> F.fprintf fmt "(Owi1 %a %a)" pp_signedness sg pp_wiop1 o
-
-(* -------------------------------------------------------------------- *)
-(* Binary operators *)
+  | Oword_of_int ws -> F.fprintf fmt "(Oword_of_int %a)" pp_wsize ws
+  | Oint_of_word (s, ws) ->
+      F.fprintf fmt "(Oint_of_word %a %a)" pp_signedness s pp_wsize ws
+  | Osignext (szo, szi) ->
+      F.fprintf fmt "(Osignext %a %a)" pp_wsize szo pp_wsize szi
+  | Ozeroext (szo, szi) ->
+      F.fprintf fmt "(Ozeroext %a %a)" pp_wsize szo pp_wsize szi
+  | Onot -> F.fprintf fmt "Onot"
+  | Olnot ws -> F.fprintf fmt "(Olnot %a)" pp_wsize ws
+  | Oneg k -> F.fprintf fmt "(Oneg %a)" pp_op_kind k
+  | Owi1 (sg, o) -> F.fprintf fmt "(Owi1 %a %a)" pp_signedness sg pp_wiop1 o
 
 let pp_wiop2 fmt = function
   | WIadd -> F.fprintf fmt "WIadd"
@@ -213,406 +214,386 @@ let pp_wiop2 fmt = function
   | WImod -> F.fprintf fmt "WImod"
   | WIshl -> F.fprintf fmt "WIshl"
   | WIshr -> F.fprintf fmt "WIshr"
-  | WIeq  -> F.fprintf fmt "WIeq"
+  | WIeq -> F.fprintf fmt "WIeq"
   | WIneq -> F.fprintf fmt "WIneq"
-  | WIlt  -> F.fprintf fmt "WIlt"
-  | WIle  -> F.fprintf fmt "WIle"
-  | WIgt  -> F.fprintf fmt "WIgt"
-  | WIge  -> F.fprintf fmt "WIge"
+  | WIlt -> F.fprintf fmt "WIlt"
+  | WIle -> F.fprintf fmt "WIle"
+  | WIgt -> F.fprintf fmt "WIgt"
+  | WIge -> F.fprintf fmt "WIge"
 
 let pp_sop2 fmt = function
-  | Obeq    -> F.fprintf fmt "Obeq"
-  | Oand    -> F.fprintf fmt "Oand"
-  | Oor     -> F.fprintf fmt "Oor"
-  | Oadd k  -> F.fprintf fmt "(Oadd %a)" pp_op_kind k
-  | Omul k  -> F.fprintf fmt "(Omul %a)" pp_op_kind k
-  | Osub k  -> F.fprintf fmt "(Osub %a)" pp_op_kind k
+  | Obeq -> F.fprintf fmt "Obeq"
+  | Oand -> F.fprintf fmt "Oand"
+  | Oor -> F.fprintf fmt "Oor"
+  | Oadd k -> F.fprintf fmt "(Oadd %a)" pp_op_kind k
+  | Omul k -> F.fprintf fmt "(Omul %a)" pp_op_kind k
+  | Osub k -> F.fprintf fmt "(Osub %a)" pp_op_kind k
   | Odiv (s, k) -> F.fprintf fmt "(Odiv %a %a)" pp_signedness s pp_op_kind k
   | Omod (s, k) -> F.fprintf fmt "(Omod %a %a)" pp_signedness s pp_op_kind k
   | Oland ws -> F.fprintf fmt "(Oland %a)" pp_wsize ws
-  | Olor ws  -> F.fprintf fmt "(Olor %a)" pp_wsize ws
+  | Olor ws -> F.fprintf fmt "(Olor %a)" pp_wsize ws
   | Olxor ws -> F.fprintf fmt "(Olxor %a)" pp_wsize ws
-  | Olsr ws  -> F.fprintf fmt "(Olsr %a)" pp_wsize ws
-  | Olsl k   -> F.fprintf fmt "(Olsl %a)" pp_op_kind k
-  | Oasr k   -> F.fprintf fmt "(Oasr %a)" pp_op_kind k
-  | Oror ws  -> F.fprintf fmt "(Oror %a)" pp_wsize ws
-  | Orol ws  -> F.fprintf fmt "(Orol %a)" pp_wsize ws
-  | Oeq k    -> F.fprintf fmt "(Oeq %a)" pp_op_kind k
-  | Oneq k   -> F.fprintf fmt "(Oneq %a)" pp_op_kind k
-  | Olt k    -> F.fprintf fmt "(Olt %a)" pp_cmp_kind k
-  | Ole k    -> F.fprintf fmt "(Ole %a)" pp_cmp_kind k
-  | Ogt k    -> F.fprintf fmt "(Ogt %a)" pp_cmp_kind k
-  | Oge k    -> F.fprintf fmt "(Oge %a)" pp_cmp_kind k
+  | Olsr ws -> F.fprintf fmt "(Olsr %a)" pp_wsize ws
+  | Olsl k -> F.fprintf fmt "(Olsl %a)" pp_op_kind k
+  | Oasr k -> F.fprintf fmt "(Oasr %a)" pp_op_kind k
+  | Oror ws -> F.fprintf fmt "(Oror %a)" pp_wsize ws
+  | Orol ws -> F.fprintf fmt "(Orol %a)" pp_wsize ws
+  | Oeq k -> F.fprintf fmt "(Oeq %a)" pp_op_kind k
+  | Oneq k -> F.fprintf fmt "(Oneq %a)" pp_op_kind k
+  | Olt k -> F.fprintf fmt "(Olt %a)" pp_cmp_kind k
+  | Ole k -> F.fprintf fmt "(Ole %a)" pp_cmp_kind k
+  | Ogt k -> F.fprintf fmt "(Ogt %a)" pp_cmp_kind k
+  | Oge k -> F.fprintf fmt "(Oge %a)" pp_cmp_kind k
   | Ovadd (ve, ws) -> F.fprintf fmt "(Ovadd %a %a)" pp_velem ve pp_wsize ws
   | Ovsub (ve, ws) -> F.fprintf fmt "(Ovsub %a %a)" pp_velem ve pp_wsize ws
   | Ovmul (ve, ws) -> F.fprintf fmt "(Ovmul %a %a)" pp_velem ve pp_wsize ws
   | Ovlsr (ve, ws) -> F.fprintf fmt "(Ovlsr %a %a)" pp_velem ve pp_wsize ws
   | Ovlsl (ve, ws) -> F.fprintf fmt "(Ovlsl %a %a)" pp_velem ve pp_wsize ws
   | Ovasr (ve, ws) -> F.fprintf fmt "(Ovasr %a %a)" pp_velem ve pp_wsize ws
-  | Owi2 (sg, ws, o) -> F.fprintf fmt "(Owi2 %a %a %a)" pp_signedness sg pp_wsize ws pp_wiop2 o
-
-(* -------------------------------------------------------------------- *)
-(* N-ary operators *)
+  | Owi2 (sg, ws, o) ->
+      F.fprintf fmt "(Owi2 %a %a %a)" pp_signedness sg pp_wsize ws pp_wiop2 o
 
 let pp_combine_flags fmt = function
   | CF_LT s -> F.fprintf fmt "(CF_LT %a)" pp_signedness s
   | CF_LE s -> F.fprintf fmt "(CF_LE %a)" pp_signedness s
-  | CF_EQ   -> F.fprintf fmt "CF_EQ"
-  | CF_NEQ  -> F.fprintf fmt "CF_NEQ"
+  | CF_EQ -> F.fprintf fmt "CF_EQ"
+  | CF_NEQ -> F.fprintf fmt "CF_NEQ"
   | CF_GE s -> F.fprintf fmt "(CF_GE %a)" pp_signedness s
   | CF_GT s -> F.fprintf fmt "(CF_GT %a)" pp_signedness s
 
 let pp_opN fmt = function
   | Opack (ws, pe) -> F.fprintf fmt "(Opack %a %a)" pp_wsize ws pp_pelem pe
-  | Oarray len     -> F.fprintf fmt "(Oarray %a)" pp_positive len
+  | Oarray len -> F.fprintf fmt "(Oarray %a)" pp_positive len
   | Ocombine_flags c -> F.fprintf fmt "(Ocombine_flags %a)" pp_combine_flags c
 
 let pp_opN_safety fmt = function
-  | Ois_arr_init len  -> F.fprintf fmt "(Ois_arr_init %a)" pp_positive len
+  | Ois_arr_init len -> F.fprintf fmt "(Ois_arr_init %a)" pp_positive len
   | Ois_barr_init len -> F.fprintf fmt "(Ois_barr_init %a)" pp_positive len
 
-(* -------------------------------------------------------------------- *)
-(* Sopn *)
-
 let pp_spill_op fmt = function
-  | Pseudo_operator.Spill   -> F.fprintf fmt "Spill"
+  | Pseudo_operator.Spill -> F.fprintf fmt "Spill"
   | Pseudo_operator.Unspill -> F.fprintf fmt "Unspill"
 
 let pp_cil_atype fmt = function
   | Type.Coq_abool -> F.fprintf fmt "abool"
-  | Type.Coq_aint  -> F.fprintf fmt "aint"
+  | Type.Coq_aint -> F.fprintf fmt "aint"
   | Type.Coq_aword ws -> F.fprintf fmt "(aword %a)" pp_wsize ws
-  | Type.Coq_aarr (ws, p) -> F.fprintf fmt "(aarr %a %a)" pp_wsize ws pp_positive p
+  | Type.Coq_aarr (ws, p) ->
+      F.fprintf fmt "(aarr %a %a)" pp_wsize ws pp_positive p
 
 let pp_pseudo_operator fmt = function
   | Pseudo_operator.Ospill (o, tys) ->
-    F.fprintf fmt "(Ospill %a %a)" pp_spill_op o (pp_list pp_cil_atype) tys
+      F.fprintf fmt "(Ospill %a %a)" pp_spill_op o (pp_rocq_seq pp_cil_atype)
+        tys
   | Pseudo_operator.Ocopy (ws, p) ->
-    F.fprintf fmt "(Ocopy %a %a)" pp_wsize ws pp_positive p
+      F.fprintf fmt "(Ocopy %a %a)" pp_wsize ws pp_positive p
   | Pseudo_operator.Odeclassify ty ->
-    F.fprintf fmt "(Odeclassify %a)" pp_cil_atype ty
+      F.fprintf fmt "(Odeclassify %a)" pp_cil_atype ty
   | Pseudo_operator.Odeclassify_mem p ->
-    F.fprintf fmt "(Odeclassify_mem %a)" pp_positive p
+      F.fprintf fmt "(Odeclassify_mem %a)" pp_positive p
   | Pseudo_operator.Onop -> F.fprintf fmt "Onop"
-  | Pseudo_operator.Omulu ws ->
-    F.fprintf fmt "(Omulu %a)" pp_wsize ws
-  | Pseudo_operator.Oaddcarry ws ->
-    F.fprintf fmt "(Oaddcarry %a)" pp_wsize ws
-  | Pseudo_operator.Osubcarry ws ->
-    F.fprintf fmt "(Osubcarry %a)" pp_wsize ws
-  | Pseudo_operator.Oswap ty ->
-    F.fprintf fmt "(Oswap %a)" pp_cil_atype ty
+  | Pseudo_operator.Omulu ws -> F.fprintf fmt "(Omulu %a)" pp_wsize ws
+  | Pseudo_operator.Oaddcarry ws -> F.fprintf fmt "(Oaddcarry %a)" pp_wsize ws
+  | Pseudo_operator.Osubcarry ws -> F.fprintf fmt "(Osubcarry %a)" pp_wsize ws
+  | Pseudo_operator.Oswap ty -> F.fprintf fmt "(Oswap %a)" pp_cil_atype ty
 
 let pp_slh_op fmt = function
   | Slh_ops.SLHinit -> F.fprintf fmt "SLHinit"
   | Slh_ops.SLHupdate -> F.fprintf fmt "SLHupdate"
   | Slh_ops.SLHmove -> F.fprintf fmt "SLHmove"
-  | Slh_ops.SLHprotect ws ->
-    F.fprintf fmt "(SLHprotect %a)" pp_wsize ws
+  | Slh_ops.SLHprotect ws -> F.fprintf fmt "(SLHprotect %a)" pp_wsize ws
   | Slh_ops.SLHprotect_ptr (ws, p) ->
-    F.fprintf fmt "(SLHprotect_ptr %a %a)" pp_wsize ws pp_positive p
+      F.fprintf fmt "(SLHprotect_ptr %a %a)" pp_wsize ws pp_positive p
   | Slh_ops.SLHprotect_ptr_fail (ws, p) ->
-    F.fprintf fmt "(SLHprotect_ptr_fail %a %a)" pp_wsize ws pp_positive p
+      F.fprintf fmt "(SLHprotect_ptr_fail %a %a)" pp_wsize ws pp_positive p
 
 let pp_sopn pp_asm_op fmt = function
-  | Sopn.Opseudo_op o ->
-    F.fprintf fmt "(Opseudo_op %a)" pp_pseudo_operator o
-  | Sopn.Oslh o ->
-    F.fprintf fmt "(Oslh %a)" pp_slh_op o
-  | Sopn.Oasm o ->
-    F.fprintf fmt "(Oasm %a)" pp_asm_op o
+  | Sopn.Opseudo_op o -> F.fprintf fmt "(Opseudo_op %a)" pp_pseudo_operator o
+  | Sopn.Oslh o -> F.fprintf fmt "(Oslh %a)" pp_slh_op o
+  | Sopn.Oasm o -> F.fprintf fmt "(Oasm %a)" pp_asm_op o
 
-(* -------------------------------------------------------------------- *)
+(* -------------------------------------------------------------------------- *)
 (* Syscall *)
 
 let pp_syscall fmt (o : _ Syscall_t.syscall_t) =
   match o with
   | Syscall_t.RandomBytes (ws, n) ->
-    F.fprintf fmt "(RandomBytes (%a, %a))" pp_wsize ws pp_positive n
+      F.fprintf fmt "(RandomBytes (%a, %a))" pp_wsize ws pp_positive n
 
-(* -------------------------------------------------------------------- *)
+(* -------------------------------------------------------------------------- *)
 (* Expressions *)
 
 let rec pp_expr fmt = function
-  | Pconst z ->
-    F.fprintf fmt "(Pconst %a)" pp_z z
-
-  | Pbool b ->
-    F.fprintf fmt "(Pbool %b)" b
-
-  | Parr_init (ws, n) ->
-    F.fprintf fmt "(Parr_init %a %d)" pp_wsize ws n
-
-  | Pvar gv ->
-    F.fprintf fmt "(Pvar %a)" pp_gvar gv
-
+  | Pconst z -> F.fprintf fmt "(Pconst %a)" pp_z z
+  | Pbool b -> F.fprintf fmt "(Pbool %b)" b
+  | Parr_init (ws, n) -> F.fprintf fmt "(Parr_init %a %d)" pp_wsize ws n
+  | Pvar gv -> F.fprintf fmt "(Pvar %a)" pp_gvar gv
   | Pget (al, aa, ws, gv, e) ->
-    F.fprintf fmt "@[<hov 2>(Pget %a %a %a@ %a@ %a)@]"
-      pp_aligned al pp_arr_access aa pp_wsize ws pp_gvar gv pp_expr e
-
+      F.fprintf fmt "@[<hov 2>(Pget %a %a %a@ %a@ %a)@]" pp_aligned al
+        pp_arr_access aa pp_wsize ws pp_gvar gv pp_expr e
   | Psub (aa, ws, len, gv, e) ->
-    F.fprintf fmt "@[<hov 2>(Psub %a %a %d@ %a@ %a)@]"
-      pp_arr_access aa pp_wsize ws len pp_gvar gv pp_expr e
-
+      F.fprintf fmt "@[<hov 2>(Psub %a %a %d@ %a@ %a)@]" pp_arr_access aa
+        pp_wsize ws len pp_gvar gv pp_expr e
   | Pload (al, ws, e) ->
-    F.fprintf fmt "@[<hov 2>(Pload %a %a@ %a)@]"
-      pp_aligned al pp_wsize ws pp_expr e
-
+      F.fprintf fmt "@[<hov 2>(Pload %a %a@ %a)@]" pp_aligned al pp_wsize ws
+        pp_expr e
   | Papp1 (op, e) ->
-    F.fprintf fmt "@[<hov 2>(Papp1 %a@ %a)@]"
-      pp_sop1 op pp_expr e
-
+      F.fprintf fmt "@[<hov 2>(Papp1 %a@ %a)@]" pp_sop1 op pp_expr e
   | Papp2 (op, e1, e2) ->
-    F.fprintf fmt "@[<hov 2>(Papp2 %a@ %a@ %a)@]"
-      pp_sop2 op pp_expr e1 pp_expr e2
-
+      F.fprintf fmt "@[<hov 2>(Papp2 %a@ %a@ %a)@]" pp_sop2 op pp_expr e1
+        pp_expr e2
   | PappN (op, es) ->
-    F.fprintf fmt "@[<hov 2>(PappN %a@ %a)@]"
-      pp_opN op (pp_list pp_expr) es
-
+      F.fprintf fmt "@[<hov 2>(PappN %a@ %a)@]" pp_opN op (pp_rocq_seq pp_expr)
+        es
   | Pif (ty, e1, e2, e3) ->
-    F.fprintf fmt "@[<hov 2>(Pif %a@ %a@ %a@ %a)@]"
-      pp_atype ty pp_expr e1 pp_expr e2 pp_expr e3
+      F.fprintf fmt "@[<hov 2>(Pif %a@ %a@ %a@ %a)@]" pp_atype ty pp_expr e1
+        pp_expr e2 pp_expr e3
 
-let pp_exprs fmt es = pp_list pp_expr fmt es
+let pp_exprs fmt es = pp_rocq_seq pp_expr fmt es
 
-(* -------------------------------------------------------------------- *)
+(* -------------------------------------------------------------------------- *)
 (* Assertions *)
 
 let rec pp_eassert fmt = function
-  | Pexpr e ->
-    F.fprintf fmt "(Pexpr %a)" pp_expr e
-
+  | Pexpr e -> F.fprintf fmt "(Pexpr %a)" pp_expr e
   | PappN_safety (op, es) ->
-    F.fprintf fmt "@[<hov 2>(PappN_safety %a@ %a)@]"
-      pp_opN_safety op (pp_list pp_expr) es
-
-  | Pis_var_init x ->
-    F.fprintf fmt "(Pis_var_init %a)" pp_var_i x
-
+      F.fprintf fmt "@[<hov 2>(PappN_safety %a@ %a)@]" pp_opN_safety op
+        (pp_rocq_seq pp_expr) es
+  | Pis_var_init x -> F.fprintf fmt "(Pis_var_init %a)" pp_var_i x
   | Pis_mem_init (e1, e2) ->
-    F.fprintf fmt "@[<hov 2>(Pis_mem_init %a@ %a)@]"
-      pp_expr e1 pp_expr e2
-
+      F.fprintf fmt "@[<hov 2>(Pis_mem_init %a@ %a)@]" pp_expr e1 pp_expr e2
   | Pand (a1, a2) ->
-    F.fprintf fmt "@[<hov 2>(Pand %a@ %a)@]"
-      pp_eassert a1 pp_eassert a2
+      F.fprintf fmt "@[<hov 2>(Pand %a@ %a)@]" pp_eassert a1 pp_eassert a2
 
-let pp_assertion fmt (label, a) =
-  F.fprintf fmt "(%S, %a)" label pp_eassert a
+let pp_assertion fmt (label, a) = F.fprintf fmt "(%S, %a)" label pp_eassert a
 
-(* -------------------------------------------------------------------- *)
+(* -------------------------------------------------------------------------- *)
 (* Lvals *)
 
 let pp_lval fmt = function
-  | Lnone (_, ty) ->
-    F.fprintf fmt "(Lnone dummy_var_info %a)" pp_atype ty
-
-  | Lvar x ->
-    F.fprintf fmt "(Lvar %a)" pp_var_i x
-
+  | Lnone (_, ty) -> F.fprintf fmt "(Lnone dummy_var_info %a)" pp_atype ty
+  | Lvar x -> F.fprintf fmt "(Lvar %a)" pp_gv_var_i x
   | Lmem (al, ws, _, e) ->
-    F.fprintf fmt "@[<hov 2>(Lmem %a %a dummy_var_info@ %a)@]"
-      pp_aligned al pp_wsize ws pp_expr e
-
+      F.fprintf fmt "@[<hov 2>(Lmem %a %a dummy_var_info@ %a)@]" pp_aligned al
+        pp_wsize ws pp_expr e
   | Laset (al, aa, ws, x, e) ->
-    F.fprintf fmt "@[<hov 2>(Laset %a %a %a@ %a@ %a)@]"
-      pp_aligned al pp_arr_access aa pp_wsize ws pp_var_i x pp_expr e
-
+      F.fprintf fmt "@[<hov 2>(Laset %a %a %a@ %a@ %a)@]" pp_aligned al
+        pp_arr_access aa pp_wsize ws pp_gv_var_i x pp_expr e
   | Lasub (aa, ws, len, x, e) ->
-    F.fprintf fmt "@[<hov 2>(Lasub %a %a %d@ %a@ %a)@]"
-      pp_arr_access aa pp_wsize ws len pp_var_i x pp_expr e
+      F.fprintf fmt "@[<hov 2>(Lasub %a %a %d@ %a@ %a)@]" pp_arr_access aa
+        pp_wsize ws len pp_gv_var_i x pp_expr e
 
-let pp_lvals fmt lvs = pp_list pp_lval fmt lvs
+let pp_lvals fmt lvs = pp_rocq_seq pp_lval fmt lvs
 
-(* -------------------------------------------------------------------- *)
+(* -------------------------------------------------------------------------- *)
 (* Instructions *)
 
 let rec pp_instr_r pp_asm_op fmt = function
   | Cassgn (lv, tag, ty, e) ->
-    F.fprintf fmt "@[<hov 2>(Cassgn %a@ %a %a@ %a)@]"
-      pp_lval lv pp_assgn_tag tag pp_atype ty pp_expr e
-
+      F.fprintf fmt "@[<hov 2>(Cassgn %a@ %a %a@ %a)@]" pp_lval lv pp_assgn_tag
+        tag pp_atype ty pp_expr e
   | Copn (lvs, tag, op, es) ->
-    F.fprintf fmt "@[<hov 2>(Copn %a@ %a %a@ %a)@]"
-      pp_lvals lvs pp_assgn_tag tag (pp_sopn pp_asm_op) op pp_exprs es
-
+      F.fprintf fmt "@[<hov 2>(Copn %a@ %a %a@ %a)@]" pp_lvals lvs pp_assgn_tag
+        tag (pp_sopn pp_asm_op) op pp_exprs es
   | Csyscall (lvs, sc, es) ->
-    F.fprintf fmt "@[<hov 2>(Csyscall %a@ %a@ %a)@]"
-      pp_lvals lvs pp_syscall sc pp_exprs es
-
+      F.fprintf fmt "@[<hov 2>(Csyscall %a@ %a@ %a)@]" pp_lvals lvs pp_syscall
+        sc pp_exprs es
   | Cassert (label, a) ->
-    F.fprintf fmt "@[<hov 2>(Cassert %a)@]"
-      pp_assertion (label, a)
-
+      F.fprintf fmt "@[<hov 2>(Cassert %a)@]" pp_assertion (label, a)
   | Cif (e, c1, c2) ->
-    F.fprintf fmt "@[<v 2>(Cif %a@ %a@ %a)@]"
-      pp_expr e (pp_stmt pp_asm_op) c1 (pp_stmt pp_asm_op) c2
-
+      F.fprintf fmt "@[<v 2>(Cif %a@ %a@ %a)@]" pp_expr e (pp_stmt pp_asm_op) c1
+        (pp_stmt pp_asm_op) c2
   | Cfor (x, (dir, lo, hi), c) ->
-    F.fprintf fmt "@[<v 2>(Cfor %a (%a, %a, %a)@ %a)@]"
-      pp_var_i x pp_dir dir pp_expr lo pp_expr hi
-      (pp_stmt pp_asm_op) c
-
+      F.fprintf fmt "@[<v 2>(Cfor %a (%a, %a, %a)@ %a)@]" pp_var_i x pp_dir dir
+        pp_expr lo pp_expr hi (pp_stmt pp_asm_op) c
   | Cwhile (al, c1, e, _, c2) ->
-    F.fprintf fmt "@[<v 2>(Cwhile %a@ %a@ %a@ dummy_instr_info@ %a)@]"
-      pp_align al
-      (pp_stmt pp_asm_op) c1
-      pp_expr e
-      (pp_stmt pp_asm_op) c2
-
+      F.fprintf fmt "@[<v 2>(Cwhile %a@ %a@ %a@ dummy_instr_info@ %a)@]"
+        pp_align al (pp_stmt pp_asm_op) c1 pp_expr e (pp_stmt pp_asm_op) c2
   | Ccall (lvs, fn, es) ->
-    F.fprintf fmt "@[<hov 2>(Ccall %a@ %a@ %a)@]"
-      pp_lvals lvs pp_fn fn pp_exprs es
+      F.fprintf fmt "@[<hov 2>(Ccall %a@ %a@ %a)@]" pp_lvals lvs pp_fn fn
+        pp_exprs es
 
 and pp_instr pp_asm_op fmt i =
-  F.fprintf fmt "@[<hov 2>(MkI dummy_instr_info@ %a)@]"
-    (pp_instr_r pp_asm_op) i.i_desc
+  F.fprintf fmt "@[<hov 2>(MkI dummy_instr_info@ %a)@]" (pp_instr_r pp_asm_op)
+    i.i_desc
 
-and pp_stmt pp_asm_op fmt c =
-  pp_list (pp_instr pp_asm_op) fmt c
+and pp_stmt pp_asm_op fmt c = pp_rocq_seq (pp_instr pp_asm_op) fmt c
 
-(* -------------------------------------------------------------------- *)
+(* -------------------------------------------------------------------------- *)
+(* Variable declarations *)
+
+let pp_mk_ident fmt i = F.fprintf fmt "mkident %s" (string_of_uid i)
+
+let pp_vscope fmt k =
+  F.fprintf fmt "%s" (if k = Global then "Sglob" else "Slocal")
+
+let pp_mk_gvar fmt v =
+  F.fprintf fmt "mk_rocq_gvar %a (%a) (%a)" pp_vscope v.v_kind pp_atype v.v_ty
+    pp_mk_ident v.v_id
+
+let pp_gvar_definition fmt v =
+  pp_rocq_definition fmt pp_var v "gvar" pp_mk_gvar v
+
+let pp_vars_definition fmt = List.iter (pp_gvar_definition fmt)
+
+(* -------------------------------------------------------------------------- *)
 (* Functions *)
 
-let pp_define_vars fmt =
-  let pp_k fmt k = F.fprintf fmt "%s" (if k = Global then "mk_gvar" else "mk_lvar") in
-  Sv.iter (fun v ->
-    F.fprintf fmt "Definition %a := %a (mk_var_i (Var %a (mkident %s))).@ "
-      pp_var v
-      pp_k v.v_kind
-      pp_atype v.v_ty
-      (string_of_uid v.v_id)
-    )
+let pp_mk_fname fmt i = F.fprintf fmt "mkfname %s" (string_of_uid i)
 
-let pp_fd pp_asm_op fmt fd =
-  F.fprintf fmt "@[<v 2>{|@ ";
-  F.fprintf fmt "f_info := FunInfo.witness;@ ";
-  F.fprintf fmt "f_contract := None;@ ";
-  F.fprintf fmt "f_tyin := %a;@ " (pp_list pp_atype) fd.f_tyin;
-  F.fprintf fmt "f_params := %a;@ "
-    (pp_list (fun fmt (x : var) ->
-      F.fprintf fmt "(%a : var_i)" pp_var x)) fd.f_args;
-  F.fprintf fmt "f_body :=@ @[<v 0>%a@];@ " (pp_stmt pp_asm_op) fd.f_body;
-  F.fprintf fmt "f_tyout := %a;@ " (pp_list pp_atype) fd.f_tyout;
-  F.fprintf fmt "f_res := %a;@ "
-    (pp_list (fun fmt (x : var_i) ->
-      F.fprintf fmt "(%a : var_i)" pp_var_i x)) fd.f_ret;
-  F.fprintf fmt "f_extra := tt;@ ";
-  F.fprintf fmt "@]|}"
+let pp_fn_definition fmt fn =
+  pp_rocq_definition fmt pp_fn fn "funname" pp_mk_fname fn.fn_id
 
-let pp_define_fname fmt fn =
-  F.fprintf fmt "Definition %a := mkfunname %s.@ "
-    pp_fn fn
-    (string_of_uid fn.fn_id)
+let pp_f_sig suff fmt fn = F.fprintf fmt "%a_%s" pp_fn fn suff
+let pp_f_tyin = pp_f_sig "tyin"
+let pp_f_args = pp_f_sig "args"
+let pp_f_tyout = pp_f_sig "tyout"
+let pp_f_res = pp_f_sig "res"
+let pp_f_body = pp_f_sig "body"
 
-let pp_fds pp_asm_op fmt =
-  List.iter (fun fd ->
-    pp_define_fname fmt fd.f_name;
-    pp_define_vars fmt (vars_fc fd);
-    F.fprintf fmt "Definition fd_%a :=@ %a.@ @ "
-      pp_fn fd.f_name
-      (pp_fd pp_asm_op) fd
-  )
+let pp_f_sig_definition suff pp_xs fmt fn xs =
+  pp_rocq_definition fmt (pp_f_sig suff) fn "seq var_i" (pp_rocq_seq pp_xs) xs
+
+let pp_f_args_definition = pp_f_sig_definition "args" pp_gv_var
+let pp_f_res_definition = pp_f_sig_definition "res" pp_gv_var_i
+
+let pp_f_tyin_definition fmt fn tyin =
+  pp_rocq_definition fmt pp_f_tyin fn "seq stype" (pp_rocq_seq pp_atype) tyin
+
+let pp_f_tyout_definition fmt fn tyout =
+  pp_rocq_definition fmt pp_f_tyout fn "seq stype" (pp_rocq_seq pp_atype) tyout
+
+let pp_f_body_definition pp_asm_op fmt fn body =
+  pp_rocq_definition fmt pp_f_body fn "cmd" (pp_stmt pp_asm_op) body
+
+(* TODO fix info and contract *)
+let pp_fd fmt fd =
+  let pp_fields fmt fd =
+    F.fprintf fmt "f_info := FunInfo.witness;@ ";
+    F.fprintf fmt "f_contract := None;@ ";
+    F.fprintf fmt "f_tyin := %a;@ " pp_f_tyin fd.f_name;
+    F.fprintf fmt "f_params := %a;@ " pp_f_args fd.f_name;
+    F.fprintf fmt "f_body := %a;@ " pp_f_body fd.f_name;
+    F.fprintf fmt "f_tyout := %a;@ " pp_f_tyout fd.f_name;
+    F.fprintf fmt "f_res := %a;@ " pp_f_res fd.f_name;
+    F.fprintf fmt "f_extra := tt;"
+  in
+  pp_rocq_record pp_fields fmt fd
+
+let pp_fd_defintion fmt fd =
+  pp_rocq_definition fmt pp_fd_name fd.f_name "ufundef" pp_fd fd
+
+let pp_fd_block pp_asm_op fmt fd =
+  pp_separator fmt pp_fn fd.f_name;
+  pp_comment fmt "Local variables";
+  pp_vars_definition fmt (Sv.to_list (vars_fc fd));
+  pp_newline fmt;
+  pp_comment fmt "Signature";
+  pp_f_tyin_definition fmt fd.f_name fd.f_tyin;
+  pp_f_args_definition fmt fd.f_name fd.f_args;
+  pp_f_tyout_definition fmt fd.f_name fd.f_tyout;
+  pp_f_res_definition fmt fd.f_name fd.f_ret;
+  pp_newline fmt;
+  pp_comment fmt "Body";
+  pp_f_body_definition pp_asm_op fmt fd.f_name fd.f_body;
+  pp_newline fmt;
+  pp_fn_definition fmt fd.f_name;
+  pp_fd_defintion fmt fd
+
+let pp_fds pp_asm_op fmt = List.iter (pp_fd_block pp_asm_op fmt)
 
 (* -------------------------------------------------------------------- *)
 (* Globals *)
 
-let pp_glob fmt (x, gd) =
+let glob_bytes x p t = Conv.to_array8 x.v_ty p t |> Array.to_list
+
+let pp_glob_data fmt v = F.fprintf fmt "%a_data" pp_var v
+
+let pp_glob_arr_data fmt (x, gd) =
   match gd with
   | Global.Gword (ws, w) ->
-    F.fprintf fmt "(%a : var, @Gword %a (wrepr %a %a))"
-      pp_var x pp_wsize ws pp_wsize ws pp_z (Conv.z_of_word ws w)
+      pp_rocq_definition_gen fmt pp_glob_data x pp_word_ty ws (pp_word ws) w
   | Global.Garr (p, t) ->
-    let ws, arr = Conv.to_array x.v_ty p t in
-    let ws_bytes = int_of_ws ws / 8 in
-    let n = Array.length arr in
-    let total_bytes = n * ws_bytes in
-    (* Extract individual bytes from each word in little-endian order *)
-    let bytes = Array.make total_bytes Z.zero in
-    Array.iteri (fun i w ->
-      for b = 0 to ws_bytes - 1 do
-        let byte_val = Z.logand (Z.shift_right w (b * 8)) (Z.of_int 255) in
-        bytes.(i * ws_bytes + b) <- byte_val
-      done
-    ) arr;
-    (* Print as nested Mz.set calls *)
-    F.fprintf fmt "@[<hov 2>(%a : var,@ (@Garr %a@ {| WArray.arr_data :=@ "
-      pp_var x pp_positive p;
-    Array.iter (fun _byte_val ->
-      F.fprintf fmt "(Mz.set@ "
-    ) bytes;
-    F.fprintf fmt "(Mz.empty u8)";
-    Array.iteri (fun i byte_val ->
-      F.fprintf fmt "@ %a@ (wrepr U8 %a))"
-        pp_z (Z.of_int i) pp_z byte_val
-    ) bytes;
-    F.fprintf fmt "@ |}))@]"
+      let pp_bytes = pp_rocq_seq (pp_wrepr U8) in
+      pp_rocq_definition fmt pp_glob_data x "seq u8" pp_bytes (glob_bytes x p t)
 
-let globs_name name = Format.sprintf "%s_gds" (sanitize_s name)
+let pp_glob fmt (x, gd) =
+  match gd with
+  | Global.Gword _ ->
+      F.fprintf fmt "(%a, Gword %a)" pp_v_var_var x pp_glob_data x
+  | Global.Garr (p, _) ->
+      F.fprintf fmt "(%a, Garr (arr_of_bytes %a %a))" pp_v_var_var x pp_positive
+        p pp_glob_data x
 
-let pp_globs fmt name globs =
-  F.fprintf fmt "Definition %s : glob_decls := @[<v 0>%a@].@ "
-    (globs_name name)
-    (pp_list pp_glob) globs
+let pp_globs fmt name = Format.fprintf fmt "%s_gds" (sanitize_s name)
+
+let pp_globs_definition fmt name globs =
+  pp_vars_definition fmt (List.map fst globs);
+  pp_newline fmt;
+  List.iter (pp_glob_arr_data fmt) globs;
+  pp_newline fmt;
+  pp_rocq_definition fmt pp_globs name "glob_decls" (pp_rocq_seq pp_glob) globs
 
 (* -------------------------------------------------------------------------- *)
 (* Programs *)
 
-let pp_prog fmt name funcs =
+(* TODO where to get extra from? *)
+let pp_mk_prog name fmt funcs =
   let pp_fd_pair fmt fd =
     F.fprintf fmt "(%a, %a)" pp_fn fd.f_name pp_fd_name fd.f_name
   in
-  F.fprintf fmt "Definition %s : uprog :=@ @[<v 0>" (sanitize_s name);
-  F.fprintf fmt "  {|@ ";
-  F.fprintf fmt "    p_globs := %s;@ " (globs_name name);
-  F.fprintf fmt "    p_funcs := %a;@ " (pp_list pp_fd_pair) funcs;
-  F.fprintf fmt "    p_extra := tt;@ "; (* TODO where to get extra from? *)
-  F.fprintf fmt "  |}.@]@ "
+  F.fprintf fmt "p_globs := %a;@ " pp_globs name;
+  F.fprintf fmt "p_funcs := %a;@ " (pp_rocq_seq pp_fd_pair) funcs;
+  F.fprintf fmt "p_extra := tt;"
+
+let pp_prog_definition fmt name funcs =
+  pp_rocq_definition fmt F.pp_print_string (sanitize_s name) "uprog"
+    (pp_rocq_record (pp_mk_prog name))
+    funcs
 
 (* -------------------------------------------------------------------------- *)
 (* Imports *)
 
 let pp_imports fmt =
   F.fprintf fmt "From Coq Require Import ZArith.@ ";
-  F.fprintf fmt "From mathcomp Require Import ssreflect ssrbool ssrfun ssrnat eqtype seq.@ ";
-  F.fprintf fmt "@ ";
-  F.fprintf fmt "Require Import expr ident var type global pseudo_operator sopn arch_extra.@ "
+  F.fprintf fmt
+    "From mathcomp Require Import ssreflect ssrbool ssrfun ssrnat eqtype seq.@ ";
+  pp_newline fmt;
+  F.fprintf fmt
+    "Require Import expr ident var type global pseudo_operator sopn \
+     arch_extra.@ ";
+  F.fprintf fmt "Require Import jasmin_printing.@ "
 
 let pp_oracles fmt =
-  F.fprintf fmt "Require Import jasmin_printing.@ ";
   F.fprintf fmt "Axiom IdO : IdentOracles.@ ";
   F.fprintf fmt "Existing Instance IdO.@ "
 
 (* Needs ident oracles *)
 let pp_arch_imports fmt = function
   | X86_64 ->
-    F.fprintf fmt "Require Import x86_decl x86_instr_decl x86_extra.@ ";
-    F.fprintf fmt "Existing Instance x86_atoI.@ "
+      F.fprintf fmt "Require Import x86_decl x86_instr_decl x86_extra.@ ";
+      F.fprintf fmt "Existing Instance x86_atoI.@ "
   | ARM_M4 -> assert false (* TODO *)
   | RISCV -> assert false (* TODO *)
 
 (* -------------------------------------------------------------------------- *)
 (* Entry point *)
 
-let extract ?(imports=true) ?(split=false)
-    arch _pd _msfsz _asmOp pp_asm_op (gd, funcs) name fmt =
-  ignore imports; ignore split;
+let extract ?(imports = true) arch _pd _msfsz _asmOp pp_asm_op (gd, funcs) name
+    fmt =
+  ignore imports;
   F.fprintf fmt "@[<v 0>";
   pp_imports fmt;
-  F.fprintf fmt "@ ";
+  pp_newline fmt;
   pp_oracles fmt;
-  F.fprintf fmt "@ ";
+  pp_newline fmt;
   pp_arch_imports fmt arch;
-  F.fprintf fmt "@ ";
-  (* ------------------------------------------------ *)
-  (* TODO isn't this coercion defined somewhere? *)
-  F.fprintf fmt "Coercion gv : gvar >-> var_i.";
-  F.fprintf fmt "@ ";
-  (* ------------------------------------------------ *)
+  pp_newline fmt;
   pp_fds pp_asm_op fmt (List.rev funcs);
-  F.fprintf fmt "@ ";
-  pp_globs fmt name gd;
-  F.fprintf fmt "@ ";
-  pp_prog fmt name funcs;
+  pp_newline fmt;
+  pp_separator_s fmt "Globals";
+  pp_globs_definition fmt name gd;
+  pp_newline fmt;
+  pp_separator_s fmt "Program";
+  pp_prog_definition fmt name funcs;
   F.fprintf fmt "@]"
