compiler/src/toRocq.mli
@@ -1,47 +1,16 @@
-val pp_option :
-  (Format.formatter -> 'a -> unit) ->
-  Format.formatter ->
-  'a option ->
-  unit
+val pp_rocq_option :
+  (Format.formatter -> 'a -> unit) -> Format.formatter -> 'a option -> unit
 
-val pp_wsize :
-  Format.formatter ->
-  Wsize.wsize ->
-  unit
-
-val pp_string :
-  Format.formatter ->
-  string ->
-  unit
-
-val pp_bare :
-  string ->
-  Format.formatter ->
-  unit
-
-val pp_with_ws :
-  string ->
-  Format.formatter ->
-  Wsize.wsize ->
-  unit
+val pp_wsize : Format.formatter -> Wsize.wsize -> unit
+val pp_string : Format.formatter -> string -> unit
+val pp_bare : string -> Format.formatter -> unit
+val pp_with_ws : string -> Format.formatter -> Wsize.wsize -> unit
 
 val pp_with_ws2 :
-  string ->
-  Format.formatter ->
-  Wsize.wsize * Wsize.wsize ->
-  unit
+  string -> Format.formatter -> Wsize.wsize * Wsize.wsize -> unit
 
-val pp_ve :
-  string ->
-  Format.formatter ->
-  Wsize.velem ->
-  unit
-
-val pp_ve_ws :
-  string ->
-  Format.formatter ->
-  Wsize.velem * Wsize.wsize ->
-  unit
+val pp_ve : string -> Format.formatter -> Wsize.velem -> unit
+val pp_ve_ws : string -> Format.formatter -> Wsize.velem * Wsize.wsize -> unit
 
 val pp_ve_ws_ve_ws :
   string ->
@@ -50,26 +19,31 @@ val pp_ve_ws_ve_ws :
   unit
 
 val pp_rk_ws :
-  string ->
-  Format.formatter ->
-  Wsize.reg_kind * Wsize.wsize ->
-  unit
+  string -> Format.formatter -> Wsize.reg_kind * Wsize.wsize -> unit
 
 val pp_s_ws :
-  string ->
-  Format.formatter ->
-  Wsize.signedness * Wsize.wsize ->
-  unit
+  string -> Format.formatter -> Wsize.signedness * Wsize.wsize -> unit
 
 val extract :
   ?imports:bool ->
-  ?split:bool ->
   Utils.architecture ->
   Wsize.wsize ->
   Wsize.wsize ->
-  ('reg, 'regx, 'xreg, 'rflag, 'cond, 'asm_op, 'extra_op) Arch_extra.extended_op Sopn.asmOp ->
-  (Format.formatter -> ('reg, 'regx, 'xreg, 'rflag, 'cond, 'asm_op, 'extra_op) Arch_extra.extended_op -> unit) ->
-  ('info, ('reg, 'regx, 'xreg, 'rflag, 'cond, 'asm_op, 'extra_op) Arch_extra.extended_op) Prog.prog ->
+  ('reg, 'regx, 'xreg, 'rflag, 'cond, 'asm_op, 'extra_op) Arch_extra.extended_op
+  Sopn.asmOp ->
+  (Format.formatter ->
+  ('reg, 'regx, 'xreg, 'rflag, 'cond, 'asm_op, 'extra_op) Arch_extra.extended_op ->
+  unit) ->
+  ( 'info,
+    ( 'reg,
+      'regx,
+      'xreg,
+      'rflag,
+      'cond,
+      'asm_op,
+      'extra_op )
+    Arch_extra.extended_op )
+  Prog.prog ->
   string ->
   Format.formatter ->
   unit
