compiler/tests/to-rocq/accept.ml
@@ -6,16 +6,18 @@ let path = "success"
 let find_proofs_dir () =
   let rec walk dir =
     let cand = Filename.concat dir "proofs" in
-    if Sys.file_exists cand && Sys.is_directory cand
-       && Sys.file_exists (Filename.concat cand "_CoqProject")
+    if
+      Sys.file_exists cand && Sys.is_directory cand
+      && Sys.file_exists (Filename.concat cand "_CoqProject")
     then cand
     else
       let parent = Filename.dirname dir in
       if parent = dir then begin
-        prerr_endline "Could not locate Jasmin proofs/ directory; \
-                       set JASMIN_PROOFS_DIR.";
+        prerr_endline
+          "Could not locate Jasmin proofs/ directory; set JASMIN_PROOFS_DIR.";
         exit 2
-      end else walk parent
+      end
+      else walk parent
   in
   walk (Sys.getcwd ())
 
@@ -30,15 +32,18 @@ let rocq_check vfile =
   in
   let log = Filename.temp_file "rocq" ".log" in
   let args =
-    "rocq" :: "c" ::
-    r "lang" @ r "compiler" @ r "arch" @ r "3rdparty" @ r "ssrmisc"
-    @ ["-q"; Filename.quote vfile]
+    ("rocq" :: "c" :: r "lang")
+    @ r "compiler" @ r "arch" @ r "3rdparty" @ r "ssrmisc"
+    @ [ "-q"; Filename.quote vfile ]
   in
   let cmd = String.concat " " args ^ " > " ^ Filename.quote log ^ " 2>&1" in
   let rc = Sys.command cmd in
   if rc <> 0 then begin
     let ic = open_in log in
-    (try while true do prerr_endline (input_line ic) done
+    (try
+       while true do
+         prerr_endline (input_line ic)
+       done
      with End_of_file -> ());
     close_in ic
   end;
@@ -47,9 +52,9 @@ let rocq_check vfile =
 
 let cleanup_artifacts vfile =
   let base = Filename.remove_extension vfile in
-  List.iter (fun ext ->
-    try Sys.remove (base ^ ext) with _ -> ()
-  ) [".vo"; ".vos"; ".vok"; ".glob"; ".aux"]
+  List.iter
+    (fun ext -> try Sys.remove (base ^ ext) with _ -> ())
+    [ (* TODO ".v"; *) ".vo"; ".vos"; ".vok"; ".glob"; ".aux" ]
 
 let load_and_print n name =
   Format.printf "File %s: " name;
@@ -58,9 +63,8 @@ let load_and_print n name =
   let oc = open_out out_name in
   let fmt = Format.formatter_of_out_channel oc in
   match
-    ToRocq.extract ~imports:true ~split:false
-      Utils.X86_64 Arch.reg_size Arch.msf_size Arch.asmOp
-      Arch.pp_extended_op_for_rocq p "p" fmt
+    ToRocq.extract ~imports:true Utils.X86_64 Arch.reg_size Arch.msf_size
+      Arch.asmOp Arch.pp_extended_op_for_rocq p "p" fmt
   with
   | () ->
       Format.pp_print_flush fmt ();
@@ -70,7 +74,8 @@ let load_and_print n name =
       if rc = 0 then begin
         Format.printf "OK@.";
         n
-      end else begin
+      end
+      else begin
         Format.printf "rocq failed@.";
         n + 1
       end
