proofs/compiler/jasmin_printing.v
@@ -6,18 +6,26 @@ Require Import expr ident var type global pseudo_operator sopn arch_extra.
 
 Require x86_decl x86_instr_decl x86_extra.
 Require arm_decl arm_instr_decl arm_extra.
+Require riscv_decl riscv_instr_decl riscv_extra.
+
+Definition arr_of_bytes (n : positive) (bs : seq u8) : WArray.array n :=
+  rdflt (WArray.empty _) (WArray.fill n bs).
 
 Class IdentOracles :=
   {
     mkident : Z -> Ident.ident;
     mkident_inj : injective mkident;
-    mkfunname : Z -> funname;
+    mkfname : Z -> funname;
   }.
 
 Section WITH_IDO.
 
 Context {IdO : IdentOracles}.
 
+Definition mk_rocq_gvar (s : v_scope) (t : atype) (i : Ident.ident) : gvar :=
+  {| gs := s; gv := mk_var_i {| vtype := t; vname := i; |}; |}.
+
+(* TODO generalize to any fintype *)
 Section X86_ATOI.
 
 Import x86_decl x86_instr_decl x86_extra.
@@ -26,7 +34,16 @@ Definition x86_reg_to_ident (r : register) : Ident.ident :=
   mkident (Z.of_nat (find (pred1 r) cenum)).
 
 Lemma x86_reg_inj_to_ident : injective x86_reg_to_ident.
-Proof. by move=> r1 r2 /mkident_inj /Nat2Z.inj; case: r1; case: r2. Qed.
+Proof.
+  move=> r1 r2 /mkident_inj /Nat2Z.inj h.
+  (* TODO separate lemma for any fintype *)
+  have Hr1 : has (pred1 r1) (cenum : seq register)
+    by rewrite has_pred1; exact: mem_cenum r1.
+  have Hr2 : has (pred1 r2) (cenum : seq register)
+    by rewrite has_pred1; exact: mem_cenum r2.
+  by rewrite -(eqP (nth_find r1 Hr1)) (congr1 (nth r1 cenum) h)
+             (eqP (nth_find r1 Hr2)).
+Qed.
 
 Definition x86_toI_r : ToIdent register :=
   {|
@@ -36,8 +53,84 @@ Definition x86_toI_r : ToIdent register :=
     of_identE := fun _ => erefl;
   |}.
 
-Definition x86_atoI : arch_toIdent.
-Admitted.
+Definition x86_reg_ext_to_ident (rx : register_ext) : Ident.ident :=
+  mkident (Z.of_nat (size (cenum : seq register) + find (pred1 rx) cenum)).
+
+Lemma x86_reg_ext_inj_to_ident : injective x86_reg_ext_to_ident.
+Proof.
+  move=> r1 r2 /mkident_inj /Nat2Z.inj /addnI h.
+  have Hr1 : has (pred1 r1) (cenum : seq register_ext)
+    by rewrite has_pred1; exact: mem_cenum r1.
+  have Hr2 : has (pred1 r2) (cenum : seq register_ext)
+    by rewrite has_pred1; exact: mem_cenum r2.
+  by rewrite -(eqP (nth_find r1 Hr1)) (congr1 (nth r1 cenum) h)
+             (eqP (nth_find r1 Hr2)).
+Qed.
+
+Definition x86_toI_rx : ToIdent register_ext :=
+  {|
+    to_ident := x86_reg_ext_to_ident;
+    of_ident := _;
+    inj_to_ident := x86_reg_ext_inj_to_ident;
+    of_identE := fun _ => erefl;
+  |}.
+
+Definition x86_xmm_to_ident (x : xmm_register) : Ident.ident :=
+  mkident (Z.of_nat (find (pred1 x) cenum)).
+
+Lemma x86_xmm_inj_to_ident : injective x86_xmm_to_ident.
+Proof.
+  move=> r1 r2 /mkident_inj /Nat2Z.inj h.
+  have Hr1 : has (pred1 r1) (cenum : seq xmm_register)
+    by rewrite has_pred1; exact: mem_cenum r1.
+  have Hr2 : has (pred1 r2) (cenum : seq xmm_register)
+    by rewrite has_pred1; exact: mem_cenum r2.
+  by rewrite -(eqP (nth_find r1 Hr1)) (congr1 (nth r1 cenum) h)
+             (eqP (nth_find r1 Hr2)).
+Qed.
+
+Definition x86_toI_x : ToIdent xmm_register :=
+  {|
+    to_ident := x86_xmm_to_ident;
+    of_ident := _;
+    inj_to_ident := x86_xmm_inj_to_ident;
+    of_identE := fun _ => erefl;
+  |}.
+
+Definition x86_rflag_to_ident (f : rflag) : Ident.ident :=
+  mkident (Z.of_nat (find (pred1 f) cenum)).
+
+Lemma x86_rflag_inj_to_ident : injective x86_rflag_to_ident.
+Proof.
+  move=> r1 r2 /mkident_inj /Nat2Z.inj h.
+  have Hr1 : has (pred1 r1) (cenum : seq rflag)
+    by rewrite has_pred1; exact: mem_cenum r1.
+  have Hr2 : has (pred1 r2) (cenum : seq rflag)
+    by rewrite has_pred1; exact: mem_cenum r2.
+  by rewrite -(eqP (nth_find r1 Hr1)) (congr1 (nth r1 cenum) h)
+             (eqP (nth_find r1 Hr2)).
+Qed.
+
+Definition x86_toI_f : ToIdent rflag :=
+  {|
+    to_ident := x86_rflag_to_ident;
+    of_ident := _;
+    inj_to_ident := x86_rflag_inj_to_ident;
+    of_identE := fun _ => erefl;
+  |}.
+
+Lemma x86_inj_toI_reg_regx (r : register) (rx : register_ext) :
+  to_ident (ToIdent := x86_toI_r) r <> to_ident (ToIdent := x86_toI_rx) rx.
+Proof. by move=> /mkident_inj /Nat2Z.inj; case: r; case: rx. Qed.
+
+Definition x86_atoI : arch_toIdent :=
+  {|
+    toI_r := x86_toI_r;
+    toI_rx := x86_toI_rx;
+    toI_x := x86_toI_x;
+    toI_f := x86_toI_f;
+    inj_toI_reg_regx := x86_inj_toI_reg_regx;
+  |}.
 
 End X86_ATOI.
 
@@ -50,7 +143,15 @@ Definition arm_reg_to_ident (r : register) : Ident.ident :=
   mkident (Z.of_nat (find (pred1 r) cenum)).
 
 Lemma arm_reg_inj_to_ident : injective arm_reg_to_ident.
-Proof. by move=> r1 r2 /mkident_inj /Nat2Z.inj; case: r1; case: r2. Qed.
+Proof.
+  move=> r1 r2 /mkident_inj /Nat2Z.inj h.
+  have Hr1 : has (pred1 r1) (cenum : seq register)
+    by rewrite has_pred1; exact: mem_cenum r1.
+  have Hr2 : has (pred1 r2) (cenum : seq register)
+    by rewrite has_pred1; exact: mem_cenum r2.
+  by rewrite -(eqP (nth_find r1 Hr1)) (congr1 (nth r1 cenum) h)
+             (eqP (nth_find r1 Hr2)).
+Qed.
 
 Definition arm_toI_r : ToIdent register :=
   {|
@@ -60,6 +161,110 @@ Definition arm_toI_r : ToIdent register :=
     of_identE := fun _ => erefl;
   |}.
 
+Definition arm_to_ident_empty : xregister -> Ident.ident.
+Proof. by case. Defined.
+
+Lemma arm_inj_empty : injective arm_to_ident_empty.
+Proof. by case. Qed.
+
+Definition arm_rflag_to_ident (f : rflag) : Ident.ident :=
+  mkident (Z.of_nat (find (pred1 f) cenum)).
+
+Lemma arm_rflag_inj_to_ident : injective arm_rflag_to_ident.
+Proof.
+  move=> r1 r2 /mkident_inj /Nat2Z.inj h.
+  have Hr1 : has (pred1 r1) (cenum : seq rflag)
+    by rewrite has_pred1; exact: mem_cenum r1.
+  have Hr2 : has (pred1 r2) (cenum : seq rflag)
+    by rewrite has_pred1; exact: mem_cenum r2.
+  by rewrite -(eqP (nth_find r1 Hr1)) (congr1 (nth r1 cenum) h)
+             (eqP (nth_find r1 Hr2)).
+Qed.
+
+Definition arm_toI_f : ToIdent rflag :=
+  {|
+    to_ident := arm_rflag_to_ident;
+    of_ident := _;
+    inj_to_ident := arm_rflag_inj_to_ident;
+    of_identE := fun _ => erefl;
+  |}.
+
+(* TODO declare as separate [ToIdent] records *)
+Definition arm_atoI : arch_toIdent.
+Proof.
+  refine {|
+    toI_r := arm_toI_r;
+    toI_rx := {| to_ident := arm_to_ident_empty;
+                 of_ident := _;
+                 inj_to_ident := arm_inj_empty;
+                 of_identE := fun _ => erefl |};
+    toI_x := {| to_ident := arm_to_ident_empty;
+                of_ident := _;
+                inj_to_ident := arm_inj_empty;
+                of_identE := fun _ => erefl |};
+    toI_f := arm_toI_f;
+    inj_toI_reg_regx := _;
+  |}.
+  by case.
+Defined.
+
 End ARM_ATOI.
+
+
+Section RISCV_ATOI.
+
+Import riscv_decl riscv_instr_decl riscv_extra.
+
+Definition riscv_reg_to_ident (r : register) : Ident.ident :=
+  mkident (Z.of_nat (find (pred1 r) cenum)).
+
+Lemma riscv_reg_inj_to_ident : injective riscv_reg_to_ident.
+Proof.
+  move=> r1 r2 /mkident_inj /Nat2Z.inj h.
+  have Hr1 : has (pred1 r1) (cenum : seq register)
+    by rewrite has_pred1; exact: mem_cenum r1.
+  have Hr2 : has (pred1 r2) (cenum : seq register)
+    by rewrite has_pred1; exact: mem_cenum r2.
+  by rewrite -(eqP (nth_find r1 Hr1)) (congr1 (nth r1 cenum) h)
+             (eqP (nth_find r1 Hr2)).
+Qed.
+
+Definition riscv_toI_r : ToIdent register :=
+  {|
+    to_ident := riscv_reg_to_ident;
+    of_ident := _;
+    inj_to_ident := riscv_reg_inj_to_ident;
+    of_identE := fun _ => erefl;
+  |}.
+
+Definition riscv_to_ident_empty : rflag -> Ident.ident.
+Proof. by case. Defined.
+
+Lemma riscv_inj_empty : injective riscv_to_ident_empty.
+Proof. by case. Qed.
+
+(* TODO declare as separate [ToIdent] records *)
+Definition riscv_atoI : arch_toIdent.
+Proof.
+  refine {|
+    toI_r := riscv_toI_r;
+    toI_rx := {| to_ident := riscv_to_ident_empty;
+                 of_ident := _;
+                 inj_to_ident := riscv_inj_empty;
+                 of_identE := fun _ => erefl |};
+    toI_x := {| to_ident := riscv_to_ident_empty;
+                of_ident := _;
+                inj_to_ident := riscv_inj_empty;
+                of_identE := fun _ => erefl |};
+    toI_f := {| to_ident := riscv_to_ident_empty;
+                of_ident := _;
+                inj_to_ident := riscv_inj_empty;
+                of_identE := fun _ => erefl |};
+    inj_toI_reg_regx := _;
+  |}.
+  by case.
+Defined.
+
+End RISCV_ATOI.
 
 End WITH_IDO.
